Replacing the node class with a datatype instead

AVLnode.dfy
@@ -2,14 +2,14 @@ class AVLnode {
     //Height of the subtree
     var height: nat
     var number: int
-    var left: AVLnode?
-    var right: AVLnode?
+    var leftNode: AVLnode?
+    var rightNode: AVLnode?
 
     constructor Create(x: int)
     {
         height := 0;
         number := x;
-        right := null;
-        left := null;
+        rightNode := null;
+        leftNode := null;
     }
 }
