AVLtree.dfy
@@ -1,43 +1,34 @@
-include "AVLnode.dfy"
+datatype AVLnode = Leaf  |  Node (leftNode: AVLnode, height: nat, number: int, rightNode: AVLnode)
 
-class AVLtree{
-
-    var root: AVLnode?;
-
-    /* Ensure the AVL tree is a binary search tree */
-    predicate BST(l:AVLnode, x:int, r:AVLnode) 
-    reads l
-    reads r
-    {
-        (forall z :: z in get_numbers(l) ==> z < x) && 
-        (forall z :: z in get_numbers(r) ==> x < z)
-    }
-
-    /* Function that returns the numbers in an AVL tree in order */
-    function get_numbers(t:AVLnode?): set<int>
-    decreases t
-    reads t
-    {
-        if t == null then
-            {}
-        else
-            get_numbers(t.left) + {t.number} + get_numbers(t.right)
-    }
-
-    function get_node_height(node:AVLnode?): nat
-    reads node
-    {
-        if(node == null) then
-             0
-         else
-            node.height
-    }
-
-    function method max (x:int, y:int): int
-    {
-        if x >= y then 
-            x
-        else
-            y
-    }		
+/* Ensure the AVL tree is a binary search tree */
+predicate BST(left:AVLnode, x:int, right:AVLnode) 
+{
+    (forall i :: i in get_numbers(left) ==> i < x) && 
+    (forall j :: j in get_numbers(right) ==> x < j)
 }
+
+/* Function that returns the numbers in an AVL tree in order */
+function get_numbers(t:AVLnode): set<int>
+decreases t
+{
+    if t == Leaf then
+        {}
+    else
+        get_numbers(t.leftNode) + {t.number} + get_numbers(t.rightNode)
+}
+
+function get_node_height(node:AVLnode): nat
+{
+    if(node == Leaf) then
+            0
+    else
+        node.height
+}
+
+function method max (x:int, y:int): int
+{
+    if x >= y then 
+        x
+    else
+        y
+}		
